Cslib.lean
@@ -49,7 +49,6 @@ public import Cslib.Foundations.Semantics.LTS.Basic
 public import Cslib.Foundations.Semantics.LTS.Bisimulation
 public import Cslib.Foundations.Semantics.LTS.Simulation
 public import Cslib.Foundations.Semantics.LTS.TraceEq
-public import Cslib.Foundations.Semantics.ReductionSystem.Basic
 public import Cslib.Foundations.Syntax.Congruence
 public import Cslib.Foundations.Syntax.Context
 public import Cslib.Foundations.Syntax.HasAlphaEquiv
